ems/ModSemFacts.v
@@ -231,7 +231,7 @@ Section COMM.
       + left. unfold trans_l, trans_r.
         rewrite ! alist_find_map. rewrite MS1, MS0. et.
     - exists tt. econs; et; clarify.
-      unfold comm_st. ss. exists (init_st ms1), (init_st ms0). et.
+      unfold comm_st. ss. exists (initial_mrs ms1), (initial_mrs ms0). et.
 Qed.
 
 End COMM.
@@ -470,7 +470,7 @@ Proof.
   unfold compile. red. 
   eapply adequacy_local_aux; et.
   2: { exists tt. instantiate (1:= top2). instantiate (1:=(fun _ => assoc_st)).  econs; et; clarify.
-       unfold assoc_st. ss. exists (init_st ms0), (init_st ms1), (init_st ms2). splits; et. }
+       unfold assoc_st. ss. exists (initial_mrs ms0), (initial_mrs ms1), (initial_mrs ms2). splits; et. }
   i. s.
   unfold add_fnsems, trans_l, trans_r. s. unfold add_fnsems, trans_l, trans_r.
   rewrite ! alist_find_app_o. rewrite ! alist_find_map.
@@ -526,7 +526,7 @@ Proof.
   unfold compile. red.
   eapply adequacy_local_aux; et.
   2: { exists tt. instantiate (1:= top2). instantiate (1:=(fun _ => assoc_rev_st)).  econs; et; clarify.
-       unfold assoc_rev_st. ss. exists (init_st ms0), (init_st ms1), (init_st ms2). splits; et. }
+       unfold assoc_rev_st. ss. exists (initial_mrs ms0), (initial_mrs ms1), (initial_mrs ms2). splits; et. }
   i. s.
   unfold add_fnsems, trans_l, trans_r. s. unfold add_fnsems, trans_l, trans_r.
   rewrite ! alist_find_app_o. rewrite ! alist_find_map.
@@ -707,7 +707,7 @@ Proof.
   unfold compile. red. 
   eapply adequacy_local_aux; et.
   2: { exists tt. instantiate (1:= top2). instantiate (1:= (fun _ => empty_st)). econs; et; clarify.
-       unfold empty_st. ss. exists (init_st ms). et. }
+       unfold empty_st. ss. exists (initial_mrs ms). et. }
   i. s.
   unfold add_fnsems, trans_l, trans_r. s.
   rewrite ! alist_find_app_o. rewrite ! alist_find_map. 
@@ -733,7 +733,7 @@ Proof.
   unfold compile. red. 
   eapply adequacy_local_aux; et.
   2: { exists tt. instantiate (1:= top2). instantiate (1:= (fun _ => empty_rev_st)). econs; et; clarify.
-       unfold empty_st. ss. exists (init_st ms). et. }
+       unfold empty_st. ss. exists (initial_mrs ms). et. }
   i. s.
   unfold add_fnsems, trans_l, trans_r. s.
   rewrite ! alist_find_app_o. rewrite ! alist_find_map. 
